<?xml version="1.0" encoding="utf-8"?>
<rdf:RDF
  xmlns:vann="http://purl.org/vocab/vann/"
  xmlns:dqv="http://www.w3.org/ns/dqv#"
  xmlns:owl="http://www.w3.org/2002/07/owl#"
  xmlns:dcterms="http://purl.org/dc/terms/"
  xmlns:rdfs="http://www.w3.org/2000/01/rdf-schema#"
  xmlns:rdf="http://www.w3.org/1999/02/22-rdf-syntax-ns#"
  xmlns:vaem="http://www.linkedmodel.org/schema/vaem#"
  xmlns:schema="https://schema.org/"
>
  <owl:DatatypeProperty rdf:about="http://w3id.org/abecto/vocabulary#keyVariableName">
    <rdfs:label xml:lang="en">key variable name</rdfs:label>
    <rdfs:comment xml:lang="en">The name of a variable that serves as primary key for an aspect.</rdfs:comment>
    <rdfs:domain rdf:resource="http://w3id.org/abecto/vocabulary#Aspect"/>
    <rdfs:range rdf:resource="http://www.w3.org/2001/XMLSchema#string"/>
    <rdfs:isDefinedBy>
      <owl:Ontology rdf:about="http://w3id.org/abecto/vocabulary">
        <owl:imports rdf:resource="http://www.w3.org/ns/dcat"/>
        <owl:imports rdf:resource="http://www.w3.org/ns/dqv"/>
        <owl:imports rdf:resource="http://www.w3.org/2016/05/ldqd"/>
        <owl:imports rdf:resource="http://www.opmw.org/p-plan.owl"/>
        <owl:imports rdf:resource="http://www.w3.org/ns/prov"/>
        <owl:imports rdf:resource="http://www.w3.org/2004/03/trix/rdfg-1/"/>
        <vaem:rationale><![CDATA[using statement `owl:imports <http://www.opmw.org/p-plan.owl>` because statement `owl:imports <http://purl.org/net/p-plan>` does not work]]></vaem:rationale>
        <vann:preferredNamespaceUri>http://w3id.org/abecto/vocabulary#</vann:preferredNamespaceUri>
        <vann:preferredNamespacePrefix>av</vann:preferredNamespacePrefix>
        <dcterms:title xml:lang="en">ABECTO Vocabulary</dcterms:title>
        <dcterms:description xml:lang="en">The ABECTO Vocabulary (AV) is a vocabulary for the description of execution plans and results of the ABox Evaluation and Comparison Tool for Ontologies (ABECTO).</dcterms:description>
        <dcterms:creator>
          <rdf:Description rdf:nodeID="nae74334857d54b70b021d66ac1ec543cb1">
            <schema:name>Jan Martin Keil</schema:name>
            <schema:identifier rdf:resource="https://orcid.org/0000-0002-7733-0193"/>
            <schema:affiliation>
              <rdf:Description rdf:nodeID="nae74334857d54b70b021d66ac1ec543cb2">
                <schema:name>Heinz Nixdorf Chair for Distributed Information Systems, Friedrich Schiller University Jena</schema:name>
                <schema:url rdf:resource="https://www.fusion.uni-jena.de/"/>
              </rdf:Description>
            </schema:affiliation>
          </rdf:Description>
        </dcterms:creator>
        <dcterms:license rdf:resource="http://creativecommons.org/licenses/by/4.0/"/>
        <dcterms:created rdf:datatype="http://www.w3.org/2001/XMLSchema#date">2022-08-17</dcterms:created>
        <dcterms:modified rdf:datatype="http://www.w3.org/2001/XMLSchema#date">2024-10-04</dcterms:modified>
        <owl:versionInfo>1.3.0</owl:versionInfo>
        <owl:versionIRI rdf:resource="http://w3id.org/abecto/vocabulary/1.3.0"/>
        <owl:priorVersion rdf:resource="http://w3id.org/abecto/vocabulary/1.2.1"/>
      </owl:Ontology>
    </rdfs:isDefinedBy>
  </owl:DatatypeProperty>
  <owl:Class rdf:about="http://w3id.org/abecto/vocabulary#ResourceDuplicate">
    <rdfs:subClassOf rdf:resource="http://w3id.org/abecto/vocabulary#QualityAnnotationBody"/>
    <rdfs:label xml:lang="en">resource omission</rdfs:label>
    <rdfs:comment xml:lang="en">An instance serves as the body (oa:hasBody) of a dqv:QualityAnnotation on a resource (oa:hasTarget). It denotes the presence of a corresponding resource (av:comparedToResource) of a specified aspect (av:affectedAspect) in the same dataset.</rdfs:comment>
    <rdfs:isDefinedBy rdf:resource="http://w3id.org/abecto/vocabulary"/>
  </owl:Class>
  <owl:DatatypeProperty rdf:about="http://w3id.org/abecto/vocabulary#value">
    <rdfs:label xml:lang="en">value</rdfs:label>
    <rdfs:comment xml:lang="en">The value of a parameter.</rdfs:comment>
    <rdfs:domain rdf:resource="http://w3id.org/abecto/vocabulary#Parameter"/>
    <rdfs:range rdf:resource="http://www.w3.org/2001/XMLSchema#string"/>
    <rdfs:isDefinedBy rdf:resource="http://w3id.org/abecto/vocabulary"/>
  </owl:DatatypeProperty>
  <owl:Class rdf:about="http://w3id.org/abecto/vocabulary#StepExecution">
    <rdfs:subClassOf rdf:resource="http://purl.org/net/p-plan#Activity"/>
    <rdfs:label xml:lang="en">step execution</rdfs:label>
    <rdfs:comment xml:lang="en">An activity that executes a single step of a plan. It is determined by the corresponding step (p-plan:correspondsToStep), start and end date time (prov:startedAtTime, prov:endedAtTime), and the used primary and meta data graphs (prov:used).</rdfs:comment>
    <rdfs:isDefinedBy rdf:resource="http://w3id.org/abecto/vocabulary"/>
  </owl:Class>
  <owl:ObjectProperty rdf:about="http://w3id.org/abecto/vocabulary#affectedAspect">
    <rdfs:label xml:lang="en">affected aspect</rdfs:label>
    <rdfs:comment xml:lang="en">The aspect that is concerned by some meta data, such as deviations, value omissions and resource omissions, quality measurements or issues.</rdfs:comment>
    <rdfs:domain>
      <owl:Class rdf:nodeID="nae74334857d54b70b021d66ac1ec543cb3">
        <owl:unionOf rdf:parseType="Collection">
          <rdf:Description rdf:about="http://w3id.org/abecto/vocabulary#QualityAnnotationBody"/>
          <rdf:Description rdf:about="http://w3id.org/abecto/vocabulary#QualityMeasurement"/>
        </owl:unionOf>
      </owl:Class>
    </rdfs:domain>
    <rdfs:range rdf:resource="http://w3id.org/abecto/vocabulary#Aspect"/>
    <rdfs:isDefinedBy rdf:resource="http://w3id.org/abecto/vocabulary"/>
  </owl:ObjectProperty>
  <owl:ObjectProperty rdf:about="http://w3id.org/abecto/vocabulary#associatedDataset">
    <rdfs:label xml:lang="en">associated dataset</rdfs:label>
    <rdfs:comment xml:lang="en">The dataset to that a resource belongs, such as primary or meta data graphs, aspect patterns or steps.</rdfs:comment>
    <rdfs:range rdf:resource="http://www.w3.org/ns/dcat#Dataset"/>
    <rdfs:seeAlso rdf:resource="http://w3id.org/abecto/vocabulary#PrimaryDataGraph"/>
    <rdfs:seeAlso rdf:resource="http://w3id.org/abecto/vocabulary#MetaDataGraph"/>
    <rdfs:seeAlso rdf:resource="http://w3id.org/abecto/vocabulary#AspectPattern"/>
    <rdfs:seeAlso rdf:resource="http://w3id.org/abecto/vocabulary#Step"/>
    <rdfs:isDefinedBy rdf:resource="http://w3id.org/abecto/vocabulary"/>
  </owl:ObjectProperty>
  <dqv:Metric rdf:about="http://w3id.org/abecto/vocabulary#deduplicatedCount">
    <rdfs:label xml:lang="en">deduplicated count</rdfs:label>
    <rdfs:comment xml:lang="en">The number of deduplicated resources or deduplicated property values of a certain aspect in a dataset.</rdfs:comment>
    <dqv:inDimension rdf:resource="http://www.w3.org/2016/05/ldqd#completeness"/>
    <rdfs:isDefinedBy rdf:resource="http://w3id.org/abecto/vocabulary"/>
  </dqv:Metric>
  <dqv:Metric rdf:about="http://w3id.org/abecto/vocabulary#count">
    <rdfs:label xml:lang="en">count</rdfs:label>
    <rdfs:comment xml:lang="en">The number of resources or property values of a certain aspect in a dataset.</rdfs:comment>
    <dqv:inDimension rdf:resource="http://www.w3.org/2016/05/ldqd#completeness"/>
    <rdfs:isDefinedBy rdf:resource="http://w3id.org/abecto/vocabulary"/>
  </dqv:Metric>
  <owl:DatatypeProperty rdf:about="http://w3id.org/abecto/vocabulary#issueType">
    <rdf:type rdf:resource="http://www.w3.org/2002/07/owl#FunctionalProperty"/>
    <rdfs:label xml:lang="en">issue type</rdfs:label>
    <rdfs:comment xml:lang="en">The described custom type of an issue.</rdfs:comment>
    <rdfs:domain rdf:resource="http://w3id.org/abecto/vocabulary#Issue"/>
    <rdfs:range rdf:resource="http://www.w3.org/2001/XMLSchema#string"/>
    <rdfs:isDefinedBy rdf:resource="http://w3id.org/abecto/vocabulary"/>
  </owl:DatatypeProperty>
  <owl:DatatypeProperty rdf:about="http://w3id.org/abecto/vocabulary#key">
    <rdfs:label xml:lang="en">key</rdfs:label>
    <rdfs:label xml:lang="en">name</rdfs:label>
    <rdfs:comment xml:lang="en">The key or name of a parameter.</rdfs:comment>
    <rdfs:domain rdf:resource="http://w3id.org/abecto/vocabulary#Parameter"/>
    <rdfs:range rdf:resource="http://www.w3.org/2001/XMLSchema#string"/>
    <rdfs:isDefinedBy rdf:resource="http://w3id.org/abecto/vocabulary"/>
  </owl:DatatypeProperty>
  <dqv:Metric rdf:about="http://w3id.org/abecto/vocabulary#absoluteCoveredness">
    <rdfs:label xml:lang="en">absolute coveredness</rdfs:label>
    <rdfs:comment xml:lang="en">The number of resources of a certain aspect in the assessed dataset for that any other dataset contains a corresponding resource.</rdfs:comment>
    <dqv:inDimension rdf:resource="http://www.w3.org/2016/05/ldqd#trustworthiness"/>
    <rdfs:isDefinedBy rdf:resource="http://w3id.org/abecto/vocabulary"/>
  </dqv:Metric>
  <owl:DatatypeProperty rdf:about="http://w3id.org/abecto/vocabulary#affectedVariableName">
    <rdfs:label xml:lang="en">affected variable name</rdfs:label>
    <rdfs:comment xml:lang="en">The variable of an aspect that is concerned by some meta data, such as deviations, value omissions, quality measurements, or issues.</rdfs:comment>
    <rdfs:domain rdf:resource="http://w3id.org/abecto/vocabulary#QualityAnnotationBody"/>
    <rdfs:range rdf:resource="http://www.w3.org/2001/XMLSchema#string"/>
    <rdfs:seeAlso rdf:resource="http://w3id.org/abecto/vocabulary#Deviation"/>
    <rdfs:seeAlso rdf:resource="http://w3id.org/abecto/vocabulary#ValueOmission"/>
    <rdfs:seeAlso rdf:resource="http://www.w3.org/ns/dqv#QualityMeasurement"/>
    <rdfs:seeAlso rdf:resource="http://w3id.org/abecto/vocabulary#Issue"/>
    <rdfs:isDefinedBy rdf:resource="http://w3id.org/abecto/vocabulary"/>
  </owl:DatatypeProperty>
  <owl:ObjectProperty rdf:about="http://w3id.org/abecto/vocabulary#predefinedMetaDataGraph">
    <rdfs:label xml:lang="en">predefined meta data graph</rdfs:label>
    <rdfs:comment xml:lang="en">A predefined meta data graph that will be taken into account during the execution of a step without being the execution result of a preceding step.</rdfs:comment>
    <rdfs:domain rdf:resource="http://w3id.org/abecto/vocabulary#Step"/>
    <rdfs:range rdf:resource="http://w3id.org/abecto/vocabulary#MetaDataGraph"/>
    <rdfs:isDefinedBy rdf:resource="http://w3id.org/abecto/vocabulary"/>
  </owl:ObjectProperty>
  <owl:ObjectProperty rdf:about="http://w3id.org/abecto/vocabulary#hasParameter">
    <rdfs:label xml:lang="en">has parameter</rdfs:label>
    <rdfs:comment xml:lang="en">A parameter that was, is, or will be involved in an execution.</rdfs:comment>
    <rdfs:range rdf:resource="http://w3id.org/abecto/vocabulary#Parameter"/>
    <rdfs:isDefinedBy rdf:resource="http://w3id.org/abecto/vocabulary"/>
  </owl:ObjectProperty>
  <owl:ObjectProperty rdf:about="http://w3id.org/abecto/vocabulary#javaClass">
    <rdfs:label xml:lang="en">processor class</rdfs:label>
    <rdfs:comment xml:lang="en"><![CDATA[The associated Java class of a processor. The value is expected to be a resource represented by an IRI with the "java" scheme and the fully qualified name of the class as path, e.g. "<java:java.util.Collection>".]]></rdfs:comment>
    <rdfs:domain rdf:resource="http://w3id.org/abecto/vocabulary#Step"/>
    <rdfs:seeAlso rdf:datatype="http://www.w3.org/2001/XMLSchema#anyURI">https://docs.oracle.com/javase/specs/jls/se16/html/jls-3.html#jls-3.8</rdfs:seeAlso>
    <rdfs:seeAlso rdf:datatype="http://www.w3.org/2001/XMLSchema#anyURI">https://docs.oracle.com/javase/specs/jls/se16/html/jls-6.html#jls-6.5.3.2</rdfs:seeAlso>
    <rdfs:seeAlso rdf:datatype="http://www.w3.org/2001/XMLSchema#anyURI">https://docs.oracle.com/javase/specs/jls/se16/html/jls-6.html#jls-6.7</rdfs:seeAlso>
    <rdfs:isDefinedBy rdf:resource="http://w3id.org/abecto/vocabulary"/>
  </owl:ObjectProperty>
  <owl:ObjectProperty rdf:about="http://w3id.org/abecto/vocabulary#comparedToDataset">
    <rdfs:label xml:lang="en">compared to dataset</rdfs:label>
    <rdfs:comment xml:lang="en">The dataset in comparison to that were derived some meta data, such as deviations, value omissions, resource omissions, or quality measurements.</rdfs:comment>
    <rdfs:domain>
      <owl:Class rdf:nodeID="nae74334857d54b70b021d66ac1ec543cb6">
        <owl:unionOf rdf:parseType="Collection">
          <rdf:Description rdf:about="http://w3id.org/abecto/vocabulary#QualityAnnotationBody"/>
          <rdf:Description rdf:about="http://w3id.org/abecto/vocabulary#QualityMeasurement"/>
        </owl:unionOf>
      </owl:Class>
    </rdfs:domain>
    <rdfs:range rdf:resource="http://www.w3.org/ns/dcat#Dataset"/>
    <rdfs:isDefinedBy rdf:resource="http://w3id.org/abecto/vocabulary"/>
  </owl:ObjectProperty>
  <dqv:Metric rdf:about="http://w3id.org/abecto/vocabulary#relativeCoveredness">
    <rdfs:label xml:lang="en">relative coveredness</rdfs:label>
    <rdfs:comment xml:lang="en">The ratio of resources of a certain aspect in the assessed dataset for that any other dataset contains a corresponding resource.</rdfs:comment>
    <dqv:inDimension rdf:resource="http://www.w3.org/2016/05/ldqd#trustworthiness"/>
    <rdfs:isDefinedBy rdf:resource="http://w3id.org/abecto/vocabulary"/>
  </dqv:Metric>
  <owl:DatatypeProperty rdf:about="http://w3id.org/abecto/vocabulary#valueFilterCondition">
    <rdfs:label xml:lang="en">value filter condition</rdfs:label>
    <rdfs:comment xml:lang="en">The value filter condition that was applied to the variable values before the measurement has been performed.</rdfs:comment>
    <rdfs:domain rdf:resource="http://www.w3.org/ns/dqv#QualityMeasurement"/>
    <rdfs:range rdf:resource="http://www.w3.org/2001/XMLSchema#string"/>
    <rdfs:isDefinedBy rdf:resource="http://w3id.org/abecto/vocabulary"/>
  </owl:DatatypeProperty>
  <owl:DatatypeProperty rdf:about="http://w3id.org/abecto/vocabulary#definingQuery">
    <rdfs:label xml:lang="en">defining query</rdfs:label>
    <rdfs:comment xml:lang="en">The query that defines the pattern of an aspect for a certain dataset.</rdfs:comment>
    <rdfs:domain rdf:resource="http://w3id.org/abecto/vocabulary#AspectPattern"/>
    <rdfs:range rdf:resource="http://www.w3.org/2001/XMLSchema#string"/>
    <rdfs:isDefinedBy rdf:resource="http://w3id.org/abecto/vocabulary"/>
  </owl:DatatypeProperty>
  <dqv:Metric rdf:about="http://w3id.org/abecto/vocabulary#relativeCoverage">
    <rdfs:label xml:lang="en">relative coverage</rdfs:label>
    <rdfs:comment xml:lang="en">The ratio of resources of a certain aspect in another dataset for that the assessed dataset contains a corresponding resource.</rdfs:comment>
    <dqv:inDimension rdf:resource="http://www.w3.org/2016/05/ldqd#completeness"/>
    <rdfs:isDefinedBy rdf:resource="http://w3id.org/abecto/vocabulary"/>
  </dqv:Metric>
  <owl:Class rdf:about="http://w3id.org/abecto/vocabulary#WrongValue">
    <rdfs:subClassOf rdf:resource="http://w3id.org/abecto/vocabulary#QualityAnnotationBody"/>
    <rdfs:label xml:lang="en">wrong value</rdfs:label>
    <rdfs:comment xml:lang="en">An instance serves as the body (oa:hasBody) of a dqv:QualityAnnotation on a resource (oa:hasTarget). It denotes the incorrectness of a value (av:affectedValue) of a specified variable (av:affectedVariableName) from a specified aspect (av:affectedAspect).</rdfs:comment>
    <rdfs:isDefinedBy rdf:resource="http://w3id.org/abecto/vocabulary"/>
  </owl:Class>
  <owl:DatatypeProperty rdf:about="http://w3id.org/abecto/vocabulary#variableName">
    <rdfs:label xml:lang="en">variable name</rdfs:label>
    <rdfs:comment xml:lang="en">The name of a variable the key variable of an aspect is connected with via a certain property path (av:propertyPath).</rdfs:comment>
    <rdfs:domain rdf:resource="http://w3id.org/abecto/vocabulary#VariablePath"/>
    <rdfs:range rdf:resource="http://www.w3.org/2001/XMLSchema#string"/>
    <rdfs:isDefinedBy rdf:resource="http://w3id.org/abecto/vocabulary"/>
  </owl:DatatypeProperty>
  <owl:ObjectProperty rdf:about="http://w3id.org/abecto/vocabulary#ofAspect">
    <rdfs:label xml:lang="en">of aspect</rdfs:label>
    <rdfs:comment xml:lang="en">The aspect an aspect pattern belongs to.</rdfs:comment>
    <rdfs:domain rdf:resource="http://w3id.org/abecto/vocabulary#AspectPattern"/>
    <rdfs:range rdf:resource="http://w3id.org/abecto/vocabulary#Aspect"/>
    <rdfs:isDefinedBy rdf:resource="http://w3id.org/abecto/vocabulary"/>
  </owl:ObjectProperty>
  <owl:DatatypeProperty rdf:about="http://w3id.org/abecto/vocabulary#propertyPath">
    <rdfs:label xml:lang="en">property path</rdfs:label>
    <rdfs:comment xml:lang="en">The property path that connects the key variable of an aspect to a certain variable (av:variableName).</rdfs:comment>
    <rdfs:domain rdf:resource="http://w3id.org/abecto/vocabulary#VariablePath"/>
    <rdfs:range rdf:resource="http://www.w3.org/2001/XMLSchema#string"/>
    <rdfs:isDefinedBy rdf:resource="http://w3id.org/abecto/vocabulary"/>
  </owl:DatatypeProperty>
  <owl:Class rdf:about="http://w3id.org/abecto/vocabulary#ResourceOmission">
    <rdfs:subClassOf rdf:resource="http://w3id.org/abecto/vocabulary#QualityAnnotationBody"/>
    <rdfs:label xml:lang="en">resource omission</rdfs:label>
    <rdfs:comment xml:lang="en">An instance serves as the body (oa:hasBody) of a dqv:QualityAnnotation on a dataset (oa:hasTarget). It denotes the absent of a corresponding resource from a specified aspect (av:affectedAspect) in comparison to a resource (av:comparedToResource) from a specified dataset (av:comparedToDataset).</rdfs:comment>
    <rdfs:isDefinedBy rdf:resource="http://w3id.org/abecto/vocabulary"/>
  </owl:Class>
  <owl:DatatypeProperty rdf:about="http://w3id.org/abecto/vocabulary#affectedValue">
    <rdfs:label xml:lang="en">affected value</rdfs:label>
    <rdfs:comment xml:lang="en">The variable value of a resource of an aspect that is concerned by some meta data, such as deviations or issues.</rdfs:comment>
    <rdfs:domain rdf:resource="http://w3id.org/abecto/vocabulary#QualityAnnotationBody"/>
    <rdfs:isDefinedBy rdf:resource="http://w3id.org/abecto/vocabulary"/>
  </owl:DatatypeProperty>
  <dqv:Metric rdf:about="http://w3id.org/abecto/vocabulary#duplicateCount">
    <rdfs:label xml:lang="en">duplicate count</rdfs:label>
    <rdfs:comment xml:lang="en">The number of duplicated resources or duplicated property values of a certain aspect in a dataset.</rdfs:comment>
    <dqv:inDimension rdf:resource="http://www.w3.org/2016/05/ldqd#conciseness"/>
    <rdfs:isDefinedBy rdf:resource="http://w3id.org/abecto/vocabulary"/>
  </dqv:Metric>
  <dqv:Metric rdf:about="http://w3id.org/abecto/vocabulary#marCompletenessThomas08">
    <rdfs:label xml:lang="en">mark and recapture</rdfs:label>
    <rdfs:comment xml:lang="en">The ratio of the completeness of a dataset compared to multiple other datasets regarding a certain aspect estimated using the mark and recapture method as defined in Paul Thomas, 2008, Generalising multiple capture-recapture to non-uniform sample sizes, https://doi.org/10.1145/1390334.1390531.</rdfs:comment>
    <dqv:inDimension rdf:resource="http://www.w3.org/2016/05/ldqd#completeness"/>
    <rdfs:seeAlso rdf:resource="https://doi.org/10.1145/1390334.1390531"/>
    <rdfs:isDefinedBy rdf:resource="http://w3id.org/abecto/vocabulary"/>
  </dqv:Metric>
  <owl:Class rdf:about="http://w3id.org/abecto/vocabulary#Plan">
    <rdfs:subClassOf rdf:resource="http://purl.org/net/p-plan#Plan"/>
    <rdfs:label xml:lang="en">ABECTO plan</rdfs:label>
    <rdfs:comment xml:lang="en">An ABECTO execution plan.</rdfs:comment>
    <rdfs:isDefinedBy rdf:resource="http://w3id.org/abecto/vocabulary"/>
  </owl:Class>
  <owl:ObjectProperty rdf:about="http://w3id.org/abecto/vocabulary#comparedToResource">
    <rdfs:label xml:lang="en">compared to resource</rdfs:label>
    <rdfs:comment xml:lang="en">The resource in comparison to that were derived some meta data, such as deviations, value omissions or resource omissions.</rdfs:comment>
    <rdfs:domain rdf:resource="http://w3id.org/abecto/vocabulary#QualityAnnotationBody"/>
    <rdfs:isDefinedBy rdf:resource="http://w3id.org/abecto/vocabulary"/>
  </owl:ObjectProperty>
  <owl:DatatypeProperty rdf:about="http://w3id.org/abecto/vocabulary#comparedToValue">
    <rdfs:label xml:lang="en">compared to value</rdfs:label>
    <rdfs:comment xml:lang="en">The value in comparison to that were derived some meta data, such as deviations, or value omissions.</rdfs:comment>
    <rdfs:domain rdf:resource="http://w3id.org/abecto/vocabulary#QualityAnnotationBody"/>
    <rdfs:isDefinedBy rdf:resource="http://w3id.org/abecto/vocabulary"/>
  </owl:DatatypeProperty>
  <dqv:Metric rdf:about="http://w3id.org/abecto/vocabulary#absoluteCoverage">
    <rdfs:label xml:lang="en">absolute coverage</rdfs:label>
    <rdfs:comment xml:lang="en">The number of resources of a certain aspect in another dataset for that the assessed dataset contains a corresponding resource.</rdfs:comment>
    <dqv:inDimension rdf:resource="http://www.w3.org/2016/05/ldqd#completeness"/>
    <rdfs:isDefinedBy rdf:resource="http://w3id.org/abecto/vocabulary"/>
  </dqv:Metric>
  <rdf:Description rdf:about="http://w3id.org/abecto/vocabulary#relevantResource">
    <owl:deprecated rdf:datatype="http://www.w3.org/2001/XMLSchema#boolean">true</owl:deprecated>
  </rdf:Description>
  <owl:Class rdf:about="http://w3id.org/abecto/vocabulary#PrimaryDataGraph">
    <rdfs:subClassOf rdf:resource="http://www.w3.org/2004/03/trix/rdfg-1/Graph"/>
    <rdfs:subClassOf rdf:resource="http://www.w3.org/ns/prov#Entity"/>
    <rdfs:label xml:lang="en">primary data graph</rdfs:label>
    <rdfs:comment xml:lang="en">A primary data graph is a RDF graph that contains primary data of a dataset (av:associatedDataset).</rdfs:comment>
    <rdfs:isDefinedBy rdf:resource="http://w3id.org/abecto/vocabulary"/>
  </owl:Class>
  <owl:Class rdf:about="http://w3id.org/abecto/vocabulary#ValueOmission">
    <rdfs:subClassOf rdf:resource="http://w3id.org/abecto/vocabulary#QualityAnnotationBody"/>
    <rdfs:label xml:lang="en">value omission</rdfs:label>
    <rdfs:comment xml:lang="en">An instance serves as the body (oa:hasBody) of a dqv:QualityAnnotation on a resource (oa:hasTarget). It denotes the absent of a certain value for a specified variable (av:affectedVariableName) from a specified aspect (av:affectedAspect) in comparison to a value (av:comparedToValue) of a corresponding resource (av:comparedToResource) from a specified dataset (av:comparedToDataset).</rdfs:comment>
    <rdfs:isDefinedBy rdf:resource="http://w3id.org/abecto/vocabulary"/>
  </owl:Class>
  <owl:Class rdf:about="http://w3id.org/abecto/vocabulary#MetaDataGraph">
    <rdfs:subClassOf rdf:resource="http://www.w3.org/ns/dqv#QualityMetadata"/>
    <rdfs:subClassOf rdf:resource="http://www.w3.org/2004/03/trix/rdfg-1/Graph"/>
    <rdfs:subClassOf rdf:resource="http://www.w3.org/ns/prov#Entity"/>
    <rdfs:label xml:lang="en">meta data graph</rdfs:label>
    <rdfs:comment xml:lang="en">A meta data graph is a RDF graph that contains meta data of a dataset (dqv:computedOn).</rdfs:comment>
    <rdfs:isDefinedBy rdf:resource="http://w3id.org/abecto/vocabulary"/>
  </owl:Class>
  <owl:Class rdf:about="http://w3id.org/abecto/vocabulary#Aspect">
    <rdfs:label xml:lang="en">aspect</rdfs:label>
    <rdfs:comment xml:lang="en">An aspect denotes a group of facts from multiple datasets belonging to corresponding features or classes of resources.</rdfs:comment>
    <rdfs:isDefinedBy rdf:resource="http://w3id.org/abecto/vocabulary"/>
  </owl:Class>
  <owl:Class rdf:about="http://w3id.org/abecto/vocabulary#AspectPattern">
    <rdfs:label xml:lang="en">aspect pattern</rdfs:label>
    <rdfs:comment xml:lang="en">An aspect pattern determines the facts from a single dataset (av:associatedDataset) belonging to a specific aspect (av:ofAspect) using a SPARQL select query (av:definingQuery).</rdfs:comment>
    <rdfs:isDefinedBy rdf:resource="http://w3id.org/abecto/vocabulary"/>
  </owl:Class>
  <owl:Class rdf:about="http://w3id.org/abecto/vocabulary#QualityAnnotationBody">
    <rdfs:label xml:lang="en">quality annotation body</rdfs:label>
    <rdfs:comment xml:lang="en">A quality annotation body is the body (oa:hasBody) of a dqv:QualityAnnotation on a resource (oa:hasTarget). This class serves as super class of different types of annotation bodies and is not intended for direct use.</rdfs:comment>
    <rdfs:isDefinedBy rdf:resource="http://w3id.org/abecto/vocabulary"/>
  </owl:Class>
  <owl:Class rdf:about="http://w3id.org/abecto/vocabulary#Issue">
    <rdfs:subClassOf rdf:resource="http://w3id.org/abecto/vocabulary#QualityAnnotationBody"/>
    <rdfs:label xml:lang="en">issue</rdfs:label>
    <rdfs:comment xml:lang="en">An instance serves as the body (oa:hasBody) of a dqv:QualityAnnotation on a resource or a dataset (oa:hasTarget). It describes an issue of a certain type (av:issueType) with a description (rdfs:comment). An issue might affect a certain aspect (av:Aspect), a certain aspect variable (av:affectedVariableName), or a certain aspect variable value (av:affectedValue).</rdfs:comment>
    <rdfs:isDefinedBy rdf:resource="http://w3id.org/abecto/vocabulary"/>
  </owl:Class>
  <owl:Class rdf:about="http://w3id.org/abecto/vocabulary#QualityMeasurement">
    <rdfs:subClassOf rdf:resource="http://www.w3.org/ns/dqv#QualityMeasurement"/>
    <rdfs:label xml:lang="en">quality measurement</rdfs:label>
    <rdfs:comment xml:lang="en">A quality measurement represents the result value (dqv:value) of an evaluation of a given dataset (dqv:computedOn) against a specific quality metric (dqv:isMeasurementOf).</rdfs:comment>
    <rdfs:isDefinedBy rdf:resource="http://w3id.org/abecto/vocabulary"/>
  </owl:Class>
  <owl:ObjectProperty rdf:about="http://w3id.org/abecto/vocabulary#correspondsToResource">
    <rdf:type rdf:resource="http://www.w3.org/2002/07/owl#SymmetricProperty"/>
    <rdf:type rdf:resource="http://www.w3.org/2002/07/owl#TransitiveProperty"/>
    <rdfs:label xml:lang="en">corresponds to resource</rdfs:label>
    <rdfs:comment xml:lang="en">A resource that corresponds to this resource.</rdfs:comment>
    <rdfs:isDefinedBy rdf:resource="http://w3id.org/abecto/vocabulary"/>
  </owl:ObjectProperty>
  <owl:ObjectProperty rdf:about="http://w3id.org/abecto/vocabulary#correspondsNotToResource">
    <rdf:type rdf:resource="http://www.w3.org/2002/07/owl#SymmetricProperty"/>
    <owl:propertyChainAxiom rdf:parseType="Collection">
      <rdf:Description rdf:about="http://w3id.org/abecto/vocabulary#correspondsNotToResource"/>
      <rdf:Description rdf:about="http://w3id.org/abecto/vocabulary#correspondsToResource"/>
    </owl:propertyChainAxiom>
    <rdfs:label xml:lang="en">corresponds not to resource</rdfs:label>
    <rdfs:comment xml:lang="en">A resource that not corresponds to this resource.</rdfs:comment>
    <rdfs:isDefinedBy rdf:resource="http://w3id.org/abecto/vocabulary"/>
  </owl:ObjectProperty>
  <owl:Class rdf:about="http://w3id.org/abecto/vocabulary#Step">
    <rdfs:subClassOf rdf:resource="http://purl.org/net/p-plan#Step"/>
    <rdfs:label xml:lang="en">step</rdfs:label>
    <rdfs:comment xml:lang="en">A single step in an ABECTO execution plan defined by the processor class, preceding steps (p-plan:isPrecededBy), parameters (av:hasParameter), and predefined meta data (av:predefinedMetaDataGraph).</rdfs:comment>
    <rdfs:isDefinedBy rdf:resource="http://w3id.org/abecto/vocabulary"/>
  </owl:Class>
  <owl:Class rdf:about="http://w3id.org/abecto/vocabulary#Parameter">
    <rdfs:label xml:lang="en">parameter</rdfs:label>
    <rdfs:comment xml:lang="en">A generic parameter defined by a key String (av:key) and a value literal (rdf:value).</rdfs:comment>
    <rdfs:isDefinedBy rdf:resource="http://w3id.org/abecto/vocabulary"/>
  </owl:Class>
  <owl:Class rdf:about="http://w3id.org/abecto/vocabulary#Deviation">
    <rdfs:subClassOf rdf:resource="http://w3id.org/abecto/vocabulary#QualityAnnotationBody"/>
    <rdfs:label xml:lang="en">deviation</rdfs:label>
    <rdfs:comment xml:lang="en">An instance serves as the body (oa:hasBody) of a dqv:QualityAnnotation on a resource (oa:hasTarget). It denotes a mismatch of the value (av:affectedValue) of a specified variable (av:affectedVariableName) from a specified aspect (av:affectedAspect) to the corresponding value (av:comparedToValue) of a corresponding resource (av:comparedToResource) from a specified dataset (av:comparedToDataset).</rdfs:comment>
    <rdfs:isDefinedBy rdf:resource="http://w3id.org/abecto/vocabulary"/>
  </owl:Class>
  <owl:Class rdf:about="http://w3id.org/abecto/vocabulary#VariablePath">
    <rdfs:label xml:lang="en">variable path</rdfs:label>
    <rdfs:comment xml:lang="en">A connection between the key variable and another variable (av:variableName) of an aspect by a property path (av:propertyPath).</rdfs:comment>
    <rdfs:isDefinedBy rdf:resource="http://w3id.org/abecto/vocabulary"/>
  </owl:Class>
</rdf:RDF>
